a version of union marshalling

lib/Marshalling/UnionMarshalling.i.dfy
@@ -1,46 +1,58 @@
 include "MarshalledAccessors.i.dfy"
 // include "../Base/sequences.i.dfy"
 
-abstract module Union2Marshalling refines Marshalling {
-  import CaseMarshalling0 : Marshalling
-  import CaseMarshalling1 : Marshalling
-  import TagMarshalling : IntegerMarshalling
-  // import Sequences
+abstract module Union2Marshalling(
+  TagInt: NativePackedInt,
+  CaseMarshalling0: Marshalling,
+  CaseMarshalling1: Marshalling)
+refines Marshalling {
+  
+  import TGM = IntegerMarshalling(TagInt)
 
   datatype UnionType = 
     | Left(l : CaseMarshalling0.UnmarshalledType)
     | Right(r: CaseMarshalling1.UnmarshalledType)
 
+  datatype Config = Config(tgmCfg: TGM.Config,
+    elemCfg0: CaseMarshalling0.Config,
+    elemCfg1: CaseMarshalling1.Config)
+
   type UnmarshalledType = UnionType
 
-  type TagType = TagMarshalling.UnmarshalledType
+  type TagType = TGM.UnmarshalledType
+
+  predicate validConfig(cfg: Config)
+  {
+    && TGM.validConfig(cfg.tgmCfg)
+    && CaseMarshalling0.validConfig(cfg.elemCfg0)
+    && CaseMarshalling1.validConfig(cfg.elemCfg1)
+  }
 
   function method getTagEnd(): uint64
   {
-    TagMarshalling.Int.Size() as uint64
+    TagInt.Size() as uint64
   }
 
-  predicate parsable(data: mseq<byte>)
+  predicate parsable(cfg: Config, data: mseq<byte>)
   {
     var tagEnd := getTagEnd() as int;
     && |data| >= tagEnd
-    && TagMarshalling.parsable(data[..tagEnd])
-    && TagMarshalling.Int.fitsInUint64(TagMarshalling.parse(data[..tagEnd]))
-    && var tag := TagMarshalling.Int.toInt(TagMarshalling.parse(data[..tagEnd]));
-    (if tag == 0 then CaseMarshalling0.parsable(data[tagEnd..])
-        else CaseMarshalling1.parsable(data[tagEnd..]))
+    && TGM.parsable(cfg.tgmCfg, data[..tagEnd])
+    && var tag := TGM.parse(cfg.tgmCfg, data[..tagEnd]);
+    (if tag == 0 then CaseMarshalling0.parsable(cfg.elemCfg0, data[tagEnd..])
+        else CaseMarshalling1.parsable(cfg.elemCfg1, data[tagEnd..]))
   }
 
-  function parse(data: mseq<byte>) : UnmarshalledType
+  function parse(cfg: Config, data: mseq<byte>) : UnmarshalledType
   {
     var tagEnd := getTagEnd() as int;
-    var tag := TagMarshalling.Int.toInt(TagMarshalling.parse(data[..tagEnd]));
+    var tag := TGM.parse(cfg.tgmCfg, data[..tagEnd]);
 
-    if tag == 0 then Left(CaseMarshalling0.parse(data[tagEnd..]))
-      else Right(CaseMarshalling1.parse(data[tagEnd..]))
+    if tag == 0 then Left(CaseMarshalling0.parse(cfg.elemCfg0, data[tagEnd..]))
+      else Right(CaseMarshalling1.parse(cfg.elemCfg1, data[tagEnd..]))
   }
 
-  method TryParse(data: mseq<byte>) returns (ovalue: Option<UnmarshalledType>)
+  method TryParse(cfg: Config, data: mseq<byte>) returns (ovalue: Option<UnmarshalledType>)
   {
     var tagEnd := getTagEnd();
 
@@ -48,34 +60,20 @@ abstract module Union2Marshalling refines Marshalling {
       return None;
     }
 
-    var tagOvalue := TagMarshalling.TryParse(data[..tagEnd]);
+    var tag :- TGM.TryParse(cfg.tgmCfg, data[..tagEnd]);
     
-    if tagOvalue.None? {
-      return None;
-    }
-
-    if !TagMarshalling.Int.fitsInUint64(tagOvalue.value) {
-      return None;
-    }
-
-    var tag := TagMarshalling.Int.toUint64(tagOvalue.value);
     ovalue := None;
 
     if tag == 0 {
-      var leftOvalue := CaseMarshalling0.TryParse(data[tagEnd..]);
-      if leftOvalue.Some? {
-        ovalue := Some(Left(leftOvalue.value));
-      }
+      var left :- CaseMarshalling0.TryParse(cfg.elemCfg0, data[tagEnd..]);
+      ovalue := Some(Left(left));
     } else {
-      var rightOvalue := CaseMarshalling1.TryParse(data[tagEnd..]);
-      if rightOvalue.Some? {
-        ovalue := Some(Right(rightOvalue.value));
-      }
+      var right :- CaseMarshalling1.TryParse(cfg.elemCfg1, data[tagEnd..]);
+      ovalue := Some(Right(right));
     }
-
   }
 
-  method Parsable(data: mseq<byte>) returns (p: bool)
+  method Parsable(cfg: Config, data: mseq<byte>) returns (p: bool)
   {
     var tagEnd := getTagEnd();
 
@@ -83,312 +81,306 @@ abstract module Union2Marshalling refines Marshalling {
       return false;
     }
 
-    var tagOvalue := TagMarshalling.TryParse(data[..tagEnd]);
+    var tagOvalue := TGM.TryParse(cfg.tgmCfg, data[..tagEnd]);
     
     if tagOvalue.None? {
       return false;
     }
 
-    if !TagMarshalling.Int.fitsInUint64(tagOvalue.value) {
-      return false;
-    }
+    var tag := TGM.Int.toUint64(tagOvalue.value);
 
-    var tag := TagMarshalling.Int.toUint64(tagOvalue.value);
+    var parsable := false;
 
     if tag == 0 {
-      p := CaseMarshalling0.Parsable(data[tagEnd..]);
+      parsable := CaseMarshalling0.Parsable(cfg.elemCfg0, data[tagEnd..]);
     } else {
-      p := CaseMarshalling1.Parsable(data[tagEnd..]);
+      parsable := CaseMarshalling1.Parsable(cfg.elemCfg1, data[tagEnd..]);
     }
+    return parsable;
   }
 
-  method Parse(data: mseq<byte>) returns (value: UnmarshalledType)
+  method Parse(cfg: Config, data: mseq<byte>) returns (value: UnmarshalledType)
   {
     var tagEnd := getTagEnd();
-    var tagOvalue := TagMarshalling.TryParse(data[..tagEnd]);
-    var tag := TagMarshalling.Int.toUint64(tagOvalue.value);
+    var tag := TGM.Parse(cfg.tgmCfg, data[..tagEnd]);
 
     if tag == 0 {
-      var leftValue := CaseMarshalling0.Parse(data[tagEnd..]);
-      value := Left(leftValue);
+      var leftValue := CaseMarshalling0.Parse(cfg.elemCfg0, data[tagEnd..]);
+      return Left(leftValue);
     } else {
-      var rightValue := CaseMarshalling1.Parse(data[tagEnd..]);
-      value := Right(rightValue);
+      var rightValue := CaseMarshalling1.Parse(cfg.elemCfg1, data[tagEnd..]);
+      return Right(rightValue);
     }
   }
 
-  predicate marshallable(value: UnmarshalledType)
+  predicate marshallable(cfg: Config, value: UnmarshalledType)
   {
-    && TagMarshalling.Int.MinValue() <= 0 < 1 < TagMarshalling.Int.UpperBound()
+    && TagInt.MinValue() <= 0 < 1 < TagInt.UpperBound()
     && match value {
-      case Left(leftValue) => CaseMarshalling0.marshallable(leftValue)
-      case Right(rightValue) => CaseMarshalling1.marshallable(rightValue)
+      case Left(leftValue) =>
+        (&& CaseMarshalling0.marshallable(cfg.elemCfg0, leftValue)
+        && getTagEnd() as nat + CaseMarshalling0.size(cfg.elemCfg0, leftValue) as nat < Uint64UpperBound())
+      case Right(rightValue) =>
+        (&& CaseMarshalling1.marshallable(cfg.elemCfg1, rightValue)
+        && getTagEnd() as nat + CaseMarshalling1.size(cfg.elemCfg1, rightValue) as nat < Uint64UpperBound())
     }
   }
 
-  function size(value: UnmarshalledType) : nat
+  function size(cfg: Config, value: UnmarshalledType) : uint64
   {
     var tagEnd := getTagEnd();
     match value {
-      case Left(leftValue) => tagEnd as nat + CaseMarshalling0.size(leftValue)
-      case Right(rightValue) => tagEnd as nat + CaseMarshalling1.size(rightValue)
+      case Left(leftValue) => tagEnd + CaseMarshalling0.size(cfg.elemCfg0, leftValue)
+      case Right(rightValue) => tagEnd + CaseMarshalling1.size(cfg.elemCfg1, rightValue)
     }
   }
 
-  method Size(value: UnmarshalledType) returns (sz: uint64)
+  method Size(cfg: Config, value: UnmarshalledType) returns (sz: uint64)
   {
     sz := getTagEnd();
-    match value
-    case Left(leftValue) => {
-      var leftSize := CaseMarshalling0.Size(leftValue);
-      sz := sz + leftSize;
+    match value {
+      case Left(leftValue) => {
+        var leftSize := CaseMarshalling0.Size(cfg.elemCfg0, leftValue);
+        sz := sz + leftSize;
+      }
+      case Right(rightValue) => {
+        var rightSize := CaseMarshalling1.Size(cfg.elemCfg1, rightValue);
+        sz := sz + rightSize;
+      }
     }
-    case Right(rightValue) => {
-      var rightSize := CaseMarshalling1.Size(rightValue);
-      sz := sz + rightSize;
-    }
+    return sz;
   }
 
-  method Marshall(value: UnmarshalledType, linear data: mseq<byte>, start: uint64)
-    returns (linear newdata: mseq<byte>, end: uint64)
+  method Marshall(cfg: Config, value: UnmarshalledType, linear inout data: mseq<byte>, start: uint64) returns (end: uint64)
   {
     ghost var tagEnd : uint64 := getTagEnd();
 
     match value
     case Left(leftValue) => {
-      newdata, end := TagMarshalling.Marshall(TagMarshalling.Int.fromUint64(0), data, start);
-      ghost var newdata1 :seq<byte>, end1 := newdata, end;
-      newdata, end := CaseMarshalling0.Marshall(leftValue, newdata, end);
+      end := TGM.Marshall(cfg.tgmCfg, 0, inout data, start);
+      ghost var newdata1 :seq<byte>, end1 := data, end;
+      end := CaseMarshalling0.Marshall(cfg.elemCfg0, leftValue, inout data, end);
 
-      assert newdata1[start..end1] == newdata[start..end1];
-      ghost var tag := TagMarshalling.Int.toInt(TagMarshalling.parse(newdata[start..end1]));
-      TagMarshalling.Int.fromtoInverses();
-      assert tag == 0;
-
-      assert newdata[start..end][..tagEnd] == newdata[start..end1];
+      assert newdata1[start..end1] == data[start..end1];
+      assert data[start..end][..tagEnd] == data[start..end1];
     }
     case Right(rightValue) => {
-      newdata, end := TagMarshalling.Marshall(TagMarshalling.Int.fromUint64(1), data, start);
-      ghost var newdata1 :seq<byte>, end1 := newdata, end;
-      newdata, end := CaseMarshalling1.Marshall(rightValue, newdata, end);
-  
-      assert newdata1[start..end1] == newdata[start..end1];
-      ghost var tag := TagMarshalling.Int.toInt(TagMarshalling.parse(newdata[start..end1]));
-      TagMarshalling.Int.fromtoInverses();
-      assert tag == 1;
+      end := TGM.Marshall(cfg.tgmCfg, 1, inout data, start);
+      ghost var newdata1 :seq<byte>, end1 := data, end;
+      end := CaseMarshalling0.Marshall(cfg.elemCfg1, rightValue, inout data, end);
 
-      assert newdata[start..end][..tagEnd] == newdata[start..end1];
+      assert newdata1[start..end1] == data[start..end1];
+      assert data[start..end][..tagEnd] == data[start..end1];
     }
   }
 }
 
+// abstract module Union3Marshalling refines Marshalling {
+//   import CaseMarshalling0 : Marshalling
+//   import CaseMarshalling1 : Marshalling
+//   import CaseMarshalling2 : Marshalling
+//   import TGM : IntegerMarshalling
+//   // import Sequences
 
-abstract module Union3Marshalling refines Marshalling {
-  import CaseMarshalling0 : Marshalling
-  import CaseMarshalling1 : Marshalling
-  import CaseMarshalling2 : Marshalling
-  import TagMarshalling : IntegerMarshalling
-  // import Sequences
+//   datatype UnionType = 
+//     | Case0(c0: CaseMarshalling0.UnmarshalledType)
+//     | Case1(c1: CaseMarshalling1.UnmarshalledType)
+//     | Case2(c2: CaseMarshalling2.UnmarshalledType)
 
-  datatype UnionType = 
-    | Case0(c0: CaseMarshalling0.UnmarshalledType)
-    | Case1(c1: CaseMarshalling1.UnmarshalledType)
-    | Case2(c2: CaseMarshalling2.UnmarshalledType)
+//   type UnmarshalledType = UnionType
 
-  type UnmarshalledType = UnionType
+//   type TagType = TGM.UnmarshalledType
 
-  type TagType = TagMarshalling.UnmarshalledType
+//   function method getTagEnd(): uint64
+//   {
+//     TGM.Int.Size() as uint64
+//   }
 
-  function method getTagEnd(): uint64
-  {
-    TagMarshalling.Int.Size() as uint64
-  }
+//   predicate parsable(data: mseq<byte>)
+//   {
+//     var tagEnd := getTagEnd() as int;
+//     && |data| >= tagEnd
+//     && TGM.parsable(data[..tagEnd])
+//     && TGM.Int.fitsInUint64(TGM.parse(data[..tagEnd]))
+//     && var tag := TGM.Int.toInt(TGM.parse(data[..tagEnd]));
+//     (if tag == 0 then CaseMarshalling0.parsable(data[tagEnd..])
+//       else if tag == 1 then CaseMarshalling1.parsable(data[tagEnd..])
+//       else CaseMarshalling2.parsable(data[tagEnd..]))
+//   }
 
-  predicate parsable(data: mseq<byte>)
-  {
-    var tagEnd := getTagEnd() as int;
-    && |data| >= tagEnd
-    && TagMarshalling.parsable(data[..tagEnd])
-    && TagMarshalling.Int.fitsInUint64(TagMarshalling.parse(data[..tagEnd]))
-    && var tag := TagMarshalling.Int.toInt(TagMarshalling.parse(data[..tagEnd]));
-    (if tag == 0 then CaseMarshalling0.parsable(data[tagEnd..])
-      else if tag == 1 then CaseMarshalling1.parsable(data[tagEnd..])
-      else CaseMarshalling2.parsable(data[tagEnd..]))
-  }
+//   function parse(data: mseq<byte>) : UnmarshalledType
+//   {
+//     var tagEnd := getTagEnd() as int;
+//     var tag := TGM.Int.toInt(TGM.parse(data[..tagEnd]));
 
-  function parse(data: mseq<byte>) : UnmarshalledType
-  {
-    var tagEnd := getTagEnd() as int;
-    var tag := TagMarshalling.Int.toInt(TagMarshalling.parse(data[..tagEnd]));
+//     if tag == 0 then Case0(CaseMarshalling0.parse(data[tagEnd..]))
+//       else if tag == 1 then Case1(CaseMarshalling1.parse(data[tagEnd..]))
+//       else Case2(CaseMarshalling2.parse(data[tagEnd..]))
+//   }
 
-    if tag == 0 then Case0(CaseMarshalling0.parse(data[tagEnd..]))
-      else if tag == 1 then Case1(CaseMarshalling1.parse(data[tagEnd..]))
-      else Case2(CaseMarshalling2.parse(data[tagEnd..]))
-  }
+//   method TryParse(data: mseq<byte>) returns (ovalue: Option<UnmarshalledType>)
+//   {
+//     var tagEnd := getTagEnd();
 
-  method TryParse(data: mseq<byte>) returns (ovalue: Option<UnmarshalledType>)
-  {
-    var tagEnd := getTagEnd();
+//     if tagEnd > |data| as uint64 {
+//       return None;
+//     }
 
-    if tagEnd > |data| as uint64 {
-      return None;
-    }
-
-    var tagOvalue := TagMarshalling.TryParse(data[..tagEnd]);
+//     var tagOvalue := TGM.TryParse(data[..tagEnd]);
     
-    if tagOvalue.None? {
-      return None;
-    }
+//     if tagOvalue.None? {
+//       return None;
+//     }
 
-    if !TagMarshalling.Int.fitsInUint64(tagOvalue.value) {
-      return None;
-    }
+//     if !TGM.Int.fitsInUint64(tagOvalue.value) {
+//       return None;
+//     }
 
-    var tag := TagMarshalling.Int.toUint64(tagOvalue.value);
-    ovalue := None;
+//     var tag := TGM.Int.toUint64(tagOvalue.value);
+//     ovalue := None;
 
-    if tag == 0 {
-      var valueOpt := CaseMarshalling0.TryParse(data[tagEnd..]);
-      if valueOpt.Some? {
-        ovalue := Some(Case0(valueOpt.value));
-      }
-    } else if tag == 1 {
-      var valueOpt := CaseMarshalling1.TryParse(data[tagEnd..]);
-      if valueOpt.Some? {
-        ovalue := Some(Case1(valueOpt.value));
-      }
-    } else {
-      var valueOpt := CaseMarshalling2.TryParse(data[tagEnd..]);
-      if valueOpt.Some? {
-        ovalue := Some(Case2(valueOpt.value));
-      }
-    }
-  }
+//     if tag == 0 {
+//       var valueOpt := CaseMarshalling0.TryParse(data[tagEnd..]);
+//       if valueOpt.Some? {
+//         ovalue := Some(Case0(valueOpt.value));
+//       }
+//     } else if tag == 1 {
+//       var valueOpt := CaseMarshalling1.TryParse(data[tagEnd..]);
+//       if valueOpt.Some? {
+//         ovalue := Some(Case1(valueOpt.value));
+//       }
+//     } else {
+//       var valueOpt := CaseMarshalling2.TryParse(data[tagEnd..]);
+//       if valueOpt.Some? {
+//         ovalue := Some(Case2(valueOpt.value));
+//       }
+//     }
+//   }
 
-  method Parsable(data: mseq<byte>) returns (p: bool)
-  {
-    var tagEnd := getTagEnd();
+//   method Parsable(data: mseq<byte>) returns (p: bool)
+//   {
+//     var tagEnd := getTagEnd();
 
-    if tagEnd > |data| as uint64 {
-      return false;
-    }
+//     if tagEnd > |data| as uint64 {
+//       return false;
+//     }
 
-    var tagOvalue := TagMarshalling.TryParse(data[..tagEnd]);
+//     var tagOvalue := TGM.TryParse(data[..tagEnd]);
     
-    if tagOvalue.None? {
-      return false;
-    }
+//     if tagOvalue.None? {
+//       return false;
+//     }
 
-    if !TagMarshalling.Int.fitsInUint64(tagOvalue.value) {
-      return false;
-    }
+//     if !TGM.Int.fitsInUint64(tagOvalue.value) {
+//       return false;
+//     }
 
-    var tag := TagMarshalling.Int.toUint64(tagOvalue.value);
+//     var tag := TGM.Int.toUint64(tagOvalue.value);
 
-    if tag == 0 {
-      p := CaseMarshalling0.Parsable(data[tagEnd..]);
-    } else if tag == 1{
-      p := CaseMarshalling1.Parsable(data[tagEnd..]);
-    } else {
-      p := CaseMarshalling2.Parsable(data[tagEnd..]);
-    }
-  }
+//     if tag == 0 {
+//       p := CaseMarshalling0.Parsable(data[tagEnd..]);
+//     } else if tag == 1{
+//       p := CaseMarshalling1.Parsable(data[tagEnd..]);
+//     } else {
+//       p := CaseMarshalling2.Parsable(data[tagEnd..]);
+//     }
+//   }
 
-  method Parse(data: mseq<byte>) returns (value: UnmarshalledType)
-  {
-    var tagEnd := getTagEnd();
-    var tagOvalue := TagMarshalling.TryParse(data[..tagEnd]);
-    var tag := TagMarshalling.Int.toUint64(tagOvalue.value);
+//   method Parse(data: mseq<byte>) returns (value: UnmarshalledType)
+//   {
+//     var tagEnd := getTagEnd();
+//     var tagOvalue := TGM.TryParse(data[..tagEnd]);
+//     var tag := TGM.Int.toUint64(tagOvalue.value);
 
-    if tag == 0 {
-      var val := CaseMarshalling0.Parse(data[tagEnd..]);
-      value := Case0(val);
-    } else if tag == 1 {
-      var val := CaseMarshalling1.Parse(data[tagEnd..]);
-      value := Case1(val);
-    } else {
-      var val := CaseMarshalling2.Parse(data[tagEnd..]);
-      value := Case2(val);    
-    }
-  }
+//     if tag == 0 {
+//       var val := CaseMarshalling0.Parse(data[tagEnd..]);
+//       value := Case0(val);
+//     } else if tag == 1 {
+//       var val := CaseMarshalling1.Parse(data[tagEnd..]);
+//       value := Case1(val);
+//     } else {
+//       var val := CaseMarshalling2.Parse(data[tagEnd..]);
+//       value := Case2(val);    
+//     }
+//   }
 
-  predicate marshallable(value: UnmarshalledType)
-  {
-    && TagMarshalling.Int.MinValue() <= 0 < 2 < TagMarshalling.Int.UpperBound()
-    && match value {
-      case Case0(c0) => CaseMarshalling0.marshallable(c0)
-      case Case1(c1) => CaseMarshalling1.marshallable(c1)
-      case Case2(c2) => CaseMarshalling2.marshallable(c2)
-    }
-  }
+//   predicate marshallable(value: UnmarshalledType)
+//   {
+//     && TGM.Int.MinValue() <= 0 < 2 < TGM.Int.UpperBound()
+//     && match value {
+//       case Case0(c0) => CaseMarshalling0.marshallable(c0)
+//       case Case1(c1) => CaseMarshalling1.marshallable(c1)
+//       case Case2(c2) => CaseMarshalling2.marshallable(c2)
+//     }
+//   }
 
-  function size(value: UnmarshalledType) : nat
-  {
-    var tagEnd := getTagEnd();
-    match value {
-      case Case0(c0) => tagEnd as nat + CaseMarshalling0.size(c0)
-      case Case1(c1) => tagEnd as nat + CaseMarshalling1.size(c1)
-      case Case2(c2) => tagEnd as nat + CaseMarshalling2.size(c2)
-    }
-  }
+//   function size(value: UnmarshalledType) : nat
+//   {
+//     var tagEnd := getTagEnd();
+//     match value {
+//       case Case0(c0) => tagEnd as nat + CaseMarshalling0.size(c0)
+//       case Case1(c1) => tagEnd as nat + CaseMarshalling1.size(c1)
+//       case Case2(c2) => tagEnd as nat + CaseMarshalling2.size(c2)
+//     }
+//   }
 
-  method Size(value: UnmarshalledType) returns (sz: uint64)
-  {
-    sz := getTagEnd();
-    match value
-    case Case0(c0) => {
-      var size := CaseMarshalling0.Size(c0);
-      sz := sz + size;
-    }
-    case Case1(c1) => {
-      var size := CaseMarshalling1.Size(c1);
-      sz := sz + size;
-    }
-    case Case2(c2) => {
-      var size := CaseMarshalling2.Size(c2);
-      sz := sz + size;
-    }
-  }
+//   method Size(value: UnmarshalledType) returns (sz: uint64)
+//   {
+//     sz := getTagEnd();
+//     match value
+//     case Case0(c0) => {
+//       var size := CaseMarshalling0.Size(c0);
+//       sz := sz + size;
+//     }
+//     case Case1(c1) => {
+//       var size := CaseMarshalling1.Size(c1);
+//       sz := sz + size;
+//     }
+//     case Case2(c2) => {
+//       var size := CaseMarshalling2.Size(c2);
+//       sz := sz + size;
+//     }
+//   }
 
-  method Marshall(value: UnmarshalledType, linear data: mseq<byte>, start: uint64)
-    returns (linear newdata: mseq<byte>, end: uint64)
-  {
-    ghost var tagEnd : uint64 := getTagEnd();
+//   method Marshall(value: UnmarshalledType, linear data: mseq<byte>, start: uint64)
+//     returns (linear newdata: mseq<byte>, end: uint64)
+//   {
+//     ghost var tagEnd : uint64 := getTagEnd();
 
-    match value
-    case Case0(c0) => {
-      newdata, end := TagMarshalling.Marshall(TagMarshalling.Int.fromUint64(0), data, start);
-      ghost var newdata1 :seq<byte>, end1 := newdata, end;
-      newdata, end := CaseMarshalling0.Marshall(c0, newdata, end);
+//     match value
+//     case Case0(c0) => {
+//       newdata, end := TGM.Marshall(TGM.Int.fromUint64(0), data, start);
+//       ghost var newdata1 :seq<byte>, end1 := newdata, end;
+//       newdata, end := CaseMarshalling0.Marshall(c0, newdata, end);
 
-      assert newdata[start..end][..tagEnd] == newdata1[start..end1] == newdata[start..end1];
-      ghost var tag := TagMarshalling.Int.toInt(TagMarshalling.parse(newdata[start..end1]));
-      TagMarshalling.Int.fromtoInverses();
-      assert tag == 0;
-    }
-    case Case1(c1) => {
-      newdata, end := TagMarshalling.Marshall(TagMarshalling.Int.fromUint64(1), data, start);
-      ghost var newdata1 :seq<byte>, end1 := newdata, end;
-      newdata, end := CaseMarshalling1.Marshall(c1, newdata, end);
+//       assert newdata[start..end][..tagEnd] == newdata1[start..end1] == newdata[start..end1];
+//       ghost var tag := TGM.Int.toInt(TGM.parse(newdata[start..end1]));
+//       TGM.Int.fromtoInverses();
+//       assert tag == 0;
+//     }
+//     case Case1(c1) => {
+//       newdata, end := TGM.Marshall(TGM.Int.fromUint64(1), data, start);
+//       ghost var newdata1 :seq<byte>, end1 := newdata, end;
+//       newdata, end := CaseMarshalling1.Marshall(c1, newdata, end);
   
-      assert newdata1[start..end1] == newdata[start..end1];
-      ghost var tag := TagMarshalling.Int.toInt(TagMarshalling.parse(newdata[start..end1]));
-      TagMarshalling.Int.fromtoInverses();
-      assert tag == 1;
+//       assert newdata1[start..end1] == newdata[start..end1];
+//       ghost var tag := TGM.Int.toInt(TGM.parse(newdata[start..end1]));
+//       TGM.Int.fromtoInverses();
+//       assert tag == 1;
 
-      assert newdata[start..end][..tagEnd] == newdata[start..end1];
-    }
-    case Case2(c2) => {
-      newdata, end := TagMarshalling.Marshall(TagMarshalling.Int.fromUint64(2), data, start);
-      ghost var newdata1 :seq<byte>, end1 := newdata, end;
-      newdata, end := CaseMarshalling2.Marshall(c2, newdata, end);
+//       assert newdata[start..end][..tagEnd] == newdata[start..end1];
+//     }
+//     case Case2(c2) => {
+//       newdata, end := TGM.Marshall(TGM.Int.fromUint64(2), data, start);
+//       ghost var newdata1 :seq<byte>, end1 := newdata, end;
+//       newdata, end := CaseMarshalling2.Marshall(c2, newdata, end);
   
-      assert newdata1[start..end1] == newdata[start..end1];
-      ghost var tag := TagMarshalling.Int.toInt(TagMarshalling.parse(newdata[start..end1]));
-      TagMarshalling.Int.fromtoInverses();
-      assert tag == 2;
+//       assert newdata1[start..end1] == newdata[start..end1];
+//       ghost var tag := TGM.Int.toInt(TGM.parse(newdata[start..end1]));
+//       TGM.Int.fromtoInverses();
+//       assert tag == 2;
 
-      assert newdata[start..end][..tagEnd] == newdata[start..end1];
-    }
-  }
-}
+//       assert newdata[start..end][..tagEnd] == newdata[start..end1];
+//     }
+//   }
+// }
